# Calculus I: Chain Rule <br> Manhattan College Interview Presentation 

Ivan E. Perez

August 4, 2021

## Presentation Outline

(1) Assumed/Preliminary Knowledge
(2) Main Lesson
(3) Examples

## Assumed/Preliminary Knowledge

The course is taught from James Stewart's Calculus: Early Transcendentals $9^{\text {th }}$ ed
Students have covered Chapter 2 (Limits and Derivatives) and Chapter 3.1-3.3.

The knowledge from chapter 2 that will be applied today will be

- Chapter 2
(1) 2.7 Derivatives and Rates of Change
(2) 2.8 Derivatives as a Function
- Chapter 3
(1) 3.1 Derivatives of Polynomials and Exponential Functions
(2) 3.2 The Product and Quotient Rules
(3)3.3 Derivatives of Trigonometric Functions


## What is The Chain Rule?

Let $u=g(x)$ be a differentiable function of $x$.
Let $f(u)$ be a differentiable function of $u$.
Then the composite function $F=f \circ g$ defined by $F(x)=f(g(x))$ is differentiable at $x$ and $F^{\prime}$ is given by the product

$$
\begin{equation*}
F^{\prime}(x)=f^{\prime}(g(x)) \cdot g^{\prime}(x) \tag{1}
\end{equation*}
$$

## Example 1: Find $F^{\prime}(x)$ if $F(x)=\sqrt{x^{2}+1}$

Solution: We can break up the outer function, $f(u)=\sqrt{u}$ and the inner part, $g(x)=x^{2}+1$. The corresponding derivatives are

$$
f^{\prime}(u)=\frac{1}{2} u^{-\frac{1}{2}}, g^{\prime}(x)=2 x
$$

Substituting into Equation 1,

$$
\begin{equation*}
F^{\prime}(x)=\frac{1}{2}\left(x^{2}+1\right)^{-\frac{1}{2}} \cdot 2 x \tag{2}
\end{equation*}
$$

which simplifies to

$$
\begin{equation*}
\frac{x}{\sqrt{x^{2}+1}} \tag{3}
\end{equation*}
$$

## Intuition behind the Chain Rule

The chain rule can be intuited by relating the derivatives of related objects. Suppose driving speed, $d y / d u$, is twice as fast as my biking speed, $d u / d x$, and biking speed is $5 x$ faster than my walking speed $d y / d x$, then my driving speed is $5 \cdot 2=(d y / d u) \cdot(d u / d x)$ times faster than my walking speed ${ }^{1}$.

$$
\begin{equation*}
\frac{d y}{d x}=\frac{d y}{d u} \cdot \frac{d u}{d x} \tag{4}
\end{equation*}
$$

## Power Rule; Find $F^{\prime}(x)$, if $F(x)=\left(x^{3}-1\right)^{100}$

Solution: We can break up the outer function, $f(u)=u^{100}$ and the inner function, $g(x)=x^{3}-1$. The corresponding derivatives are

$$
f^{\prime}(u)=100 x^{99}, g^{\prime}(x)=3 x^{2}
$$

Substituting into Equation 1,

$$
\begin{equation*}
F^{\prime}(x)=100\left(x^{3}-1\right)^{99} \cdot\left(3 x^{2}\right) \tag{5}
\end{equation*}
$$

[^0]
## Examples: Daisy-chaining The Chain Rule

Find $F^{\prime}(x)$, if $F(x)=\sin (\cos (\tan (x)))$
We can break up the chain rule into 2 steps working from outer functions towards the inner functions.
(1) Let $f(u)=\sin (u), g(x)=\cos (\tan (x))$
(2) $f^{\prime}(u)=\cos (u), g^{\prime}(x)=\frac{d}{d x} \cos (\tan (x))$
(3) The first execution of the Chain Rule is

$$
\begin{equation*}
F^{\prime}(x)=\cos (\cos (\tan (x))) \cdot \frac{d}{d x} \cos (\tan (x)) \tag{6}
\end{equation*}
$$

(9) Applying the chain rule to $g^{\prime}(x)$, we
let $h(v)=\cos (v)$ and $k(x)=\tan (x)$
(3) $h^{\prime}(v)=-\sin (v), k^{\prime}(x)=-\sec ^{2}(x)$
(6) The second execution of the Chain Rule is

$$
\begin{equation*}
g^{\prime}(x)=-\sin (\tan (x)) \cdot\left(-\sec ^{2}(x)\right) \tag{7}
\end{equation*}
$$

( 3 with that, we can finally express

$$
\begin{array}{lc}
F^{\prime}(x)= & \cos (\cos (\tan (x))) \cdot(-\sin (\tan (x))) \cdot\left(-\sec ^{2}(x)\right) \\
F^{\prime}(x)= & \cos (\cos (\tan (x))) \sin (\tan (x))\left(\sec ^{2}(x)\right) \tag{9}
\end{array}
$$

## Examples: Is The Product Rule or Quotient Rule the Chain Rule?

Suppose we are tasked with finding $F^{\prime}(x)$ of $F(x)=\left(x^{3}-2 x\right)^{2}$.
(1) By the chain rule:

$$
\begin{equation*}
F^{\prime}(x)=2\left(x^{3}-2 x\right) \cdot\left(3 x^{2}-2\right) \tag{10}
\end{equation*}
$$

where,

$$
\begin{equation*}
f(u)=u^{2}, g(x)=x^{3}-2 x \tag{11}
\end{equation*}
$$

(2) By the product rule: by setting $u=v=\left(x^{3}-2 x\right)$

$$
\begin{align*}
F^{\prime}(x)=u^{\prime} v+v^{\prime} u & =(3 x-2)\left(x^{3}-2 x\right)+(3 x-2)\left(x^{3}-2 x\right)  \tag{12}\\
& =2\left(x^{3}-2 x\right)(3 x-2) \tag{13}
\end{align*}
$$

Would the Quotient Rule Show Similar behavior?
Try finding $F^{\prime}(x)$ for

$$
\begin{equation*}
F(x)=\frac{1}{\sqrt[3]{x^{2}+1}} \tag{14}
\end{equation*}
$$

## Examples: Using the Chain Rule with Trig. Identities

Trigonometric Identities in Chapter 3 Section 3, are difficult to memorize and intuit. Restating the Pythagorean identities can be readily memorized:

$$
\begin{align*}
\sin ^{2}(x) & =1-\cos ^{2}(x)  \tag{15}\\
\sec ^{2}(x) & =1+\tan ^{2}(x)  \tag{16}\\
\csc ^{2}(x) & =1+\cot ^{2}(x) \tag{17}
\end{align*}
$$

While Chapter 2 gives enough information to work differentiate these functions without using the Chain Rule, we can simply take $f(u)=u^{2}$ and $g(x)=\sin (x), \sec (x), \csc (x)$ respectively.

## Find $F^{\prime}(x)$ if $F(x)=\sin ^{2}(x)$

By the chain rule:

$$
\begin{align*}
& F^{\prime}(x)=2(\sin (x)) \cdot \cos (x) \text { or }  \tag{18}\\
& F^{\prime}(x)=-2(\cos (x)) \cdot(-\sin (x)) \tag{19}
\end{align*}
$$

where,

$$
\begin{equation*}
f(u)=u^{2}, g(x)=\sin (x) \text { or } \cos (x) \tag{20}
\end{equation*}
$$

## Try Equations (16) and (17) at home!

## Class Challenges Worked Out at Home

Find $F^{\prime}(x)$, if $F(x)=\left(x^{2}+1\right)^{-1 / 3}$
Let $f(u)=u^{-1 / 3}, g(x)=x^{2}+1$ such that $f^{\prime}(u)=\frac{1}{3} u^{-4 / 3}, g^{\prime}(x)=2 x$
By the Chain Rule:

$$
\begin{equation*}
F^{\prime}(x)=-\frac{1}{3}\left(x^{2}+1\right)^{-4 / 3} \cdot 2 x \tag{21}
\end{equation*}
$$

Find $F^{\prime}(x)$ if $F(x)=\sec ^{2}(x)$

$$
\begin{align*}
F^{\prime}(x) & =2(\sec (x)) \cdot \sec (x) \tan (x) \text { or }  \tag{22}\\
F^{\prime}(x) & =2(\tan (x)) \cdot\left(\sec ^{2}(x)\right)  \tag{23}\\
f(u) & =u^{2}, g(x)=\sec (x) \text { or } \tan (x) \tag{24}
\end{align*}
$$

Find $F^{\prime}(x)$ if $F(x)=\csc ^{2}(x)$

$$
\begin{array}{cc}
F^{\prime}(x) & =2(\csc (x)) \cdot(-\csc (x) \cot (x)) \text { or } \\
F^{\prime}(x) & =2(\cot (x)) \cdot\left(-\csc ^{2}(x)\right) \\
f(u) & =u^{2}, g(x)=\csc (x) \text { or } \cot (x) \tag{27}
\end{array}
$$


[^0]:    ${ }^{1}$ Note that this notation is NOT a quotient but shows how the derivative can be broken up using a intermediate variable $u$

